ViE/Buffer.lean
@@ -4,3 +4,4 @@
 
 import ViE.Buffer.Manager
 import ViE.Buffer.Content
+import ViE.Buffer.EditQueue
